WIP on AllEntriesVotesWithLogProof

raft/proof/AllEntriesVotesWithLogProof.v
@@ -1,11 +1,25 @@
 Require Import List.
+Require Import Omega.
 
 Require Import VerdiTactics.
+Require Import Util.
 Require Import Net.
+Require Import UpdateLemmas.
+Local Arguments update {_} {_} {_} _ _ _ _ : simpl never.
+
 Require Import Raft.
 Require Import RaftRefinementInterface.
+Require Import CommonTheorems.
+Require Import SpecLemmas.
+Require Import RefinementSpecLemmas.
 
 Require Import AllEntriesVotesWithLogInterface.
+Require Import LogsLeaderLogsInterface.
+Require Import AppendEntriesRequestLeaderLogsInterface.
+Require Import RefinedLogMatchingLemmasInterface.
+Require Import AllEntriesLeaderLogsTermInterface.
+Require Import LeaderLogsContiguousInterface.
+Require Import OneLeaderLogPerTermInterface.
 
 Section AllEntriesVotesWithLog.
 
@@ -13,6 +27,151 @@ Section AllEntriesVotesWithLog.
   Context {one_node_params : OneNodeParams orig_base_params}.
   Context {raft_params : RaftParams orig_base_params}.
 
+  Context {llli : logs_leaderLogs_interface}.
+  Context {aerlli : append_entries_leaderLogs_interface}.
+  Context {rlmli : refined_log_matching_lemmas_interface}.
+  Context {aellti : allEntries_leaderLogs_term_interface}.
+  Context {llci : leaderLogs_contiguous_interface}.
+  Context {ollpti : one_leaderLog_per_term_interface}.
+
+  Definition allEntries_log (net : network) : Prop :=
+    forall t e h,
+      In (t, e) (allEntries (fst (nwState net h))) ->
+      In e (log (snd (nwState net h))) \/
+      (exists t' leader ll,
+         In (t', ll) (leaderLogs (fst (nwState net leader))) /\
+         t < t' /\
+         ~ In e ll).
+
+
+  (* strategy : prove allEntries_log as inductive invariant, then
+     prove allEntries_leaderLogs inductive from that *)
+
+
+  Ltac update_destruct :=
+    match goal with
+      | [ |- context [ update _ ?y _ ?x ] ] => destruct (name_eq_dec y x)
+    end.
+
+  Ltac update_destruct_hyp :=
+    match goal with
+      | [ _ : context [ update _ ?y _ ?x ] |- _ ] => destruct (name_eq_dec y x)
+    end.
+
+  Ltac destruct_update :=
+    repeat (first [update_destruct_hyp|update_destruct]; subst; rewrite_update).
+
+  Lemma appendEntries_haveNewEntries_false :
+    forall net p t n pli plt es ci h e,
+      refined_raft_intermediate_reachable net ->
+      In p (nwPackets net) ->
+      pBody p = AppendEntries t n pli plt es ci ->
+      haveNewEntries (snd (nwState net h)) es = false ->
+      In e es ->
+      In e (log (snd (nwState net h))).
+  Proof.
+    intros.
+    unfold haveNewEntries in *. do_bool. intuition;
+      [unfold not_empty in *; break_match; subst; simpl in *; intuition; congruence|].
+    break_match; try congruence.
+    do_bool. find_apply_lem_hyp findAtIndex_elim. intuition.
+    assert (es <> nil) by (destruct es; subst; simpl in *; intuition; congruence).
+    find_eapply_lem_hyp maxIndex_non_empty.
+    break_exists. intuition.
+    find_copy_eapply_lem_hyp entries_sorted_nw_invariant; eauto.
+    match goal with
+      | H : In e es |- _ => copy_eapply maxIndex_is_max H; eauto
+    end.
+    repeat find_rewrite.
+    find_eapply_lem_hyp entries_match_nw_host_invariant; eauto.
+  Qed.
+
+  Lemma allEntries_term_sanity_invariant :
+    forall net t e h,
+      refined_raft_intermediate_reachable net ->
+      In (t, e) (allEntries (fst (nwState net h))) ->
+      t <= currentTerm (snd (nwState net h)).
+  Proof.
+    admit.
+  Qed.
+  
+  Lemma allEntries_log_append_entries :
+    refined_raft_net_invariant_append_entries allEntries_log.
+  Proof.
+    red. unfold allEntries_log in *. simpl in *. intros.
+    repeat find_higher_order_rewrite.
+    destruct_update; simpl in *;
+    [|find_apply_hyp_hyp; intuition;
+      right; break_exists_exists; intuition;
+      repeat find_higher_order_rewrite;
+      destruct_update; simpl in *;
+      eauto; rewrite update_elections_data_appendEntries_leaderLogs; eauto].
+    find_eapply_lem_hyp update_elections_data_appendEntries_allEntries_detailed; eauto.
+    intuition;
+      [|repeat find_rewrite;
+         find_eapply_lem_hyp appendEntries_haveNewEntries_false; eauto].
+    find_copy_apply_hyp_hyp.
+    intuition; [|right; break_exists_exists; intuition;
+                 repeat find_higher_order_rewrite;
+                 destruct_update; simpl in *;
+                 eauto; rewrite update_elections_data_appendEntries_leaderLogs; eauto].
+    destruct (in_dec entry_eq_dec e (log d)); intuition.
+    right.
+    find_apply_lem_hyp handleAppendEntries_log_detailed. intuition; repeat find_rewrite; intuition.
+    - subst.
+      find_copy_eapply_lem_hyp allEntries_term_sanity_invariant; eauto.
+      destruct (lt_eq_lt_dec t0 t); intuition; unfold ghost_data in *; simpl in *; try omega.
+      + find_eapply_lem_hyp append_entries_leaderLogs_invariant; eauto.
+        break_exists. break_and.
+        match goal with
+          | H : In (?t, ?ll) (leaderLogs (fst (nwState _ ?leader))) |- _ =>
+            (exists t, leader, ll)
+        end.
+        split;
+          [repeat find_higher_order_rewrite;
+            destruct_update; simpl in *;
+            eauto; rewrite update_elections_data_appendEntries_leaderLogs; eauto|];
+          split; auto.
+        intuition;
+          [break_exists; intuition;
+           find_eapply_lem_hyp leaderLogs_contiguous_invariant; eauto; omega|].
+        subst.
+        match goal with
+          | H : In _ _ -> False |- _ =>
+            apply H
+        end.
+        repeat find_rewrite.
+        intuition.
+      + subst.
+        find_eapply_lem_hyp allEntries_leaderLogs_term_invariant. intuition.
+        * subst. exfalso.
+          find_copy_eapply_lem_hyp logs_leaderLogs_invariant; eauto.
+          find_copy_eapply_lem_hyp append_entries_leaderLogs_invariant; eauto.
+          break_exists; intuition;
+          [break_exists; intuition;
+           find_eapply_lem_hyp leaderLogs_contiguous_invariant; eauto; omega|].
+          subst. clean.
+          find_eapply_lem_hyp one_leaderLog_per_term_invariant; eauto;
+          conclude_using eauto. subst.
+          match goal with
+          | H : In _ _ -> False |- _ =>
+            apply H
+          end.
+          find_copy_eapply_lem_hyp entries_sorted_invariant; eauto.
+          unfold entries_sorted in *.
+          repeat find_rewrite.
+          match goal with
+            | _ : removeAfterIndex ?l (eIndex ?e) = _ |- _ =>
+              assert (In e (removeAfterIndex l (eIndex e))) by
+                  (eapply removeAfterIndex_le_In; eauto)
+          end.
+          repeat find_rewrite.
+          do_in_app; intuition.
+          assert (exists e', eIndex e' = eIndex e /\ In e' (x1 ++ x4)).
+          eapply entries_contiguous_nw_invariant; eauto.
+          intuition; [eapply entries_contiguous_invariant; eauto|].
+  Admitted.
+        
   Instance aevwli : allEntries_votesWithLog_interface.
   Admitted.
 End AllEntriesVotesWithLog.
